theories/Compositional_Structures/Basic_Modules/Condorcet_Module_Ref.thy
@@ -11,12 +11,12 @@ begin
 
 definition condorcet_score_ref :: "'a::{default, heap, hashable} Evaluation_Function_Ref" where
   "condorcet_score_ref x A p = do {
-    is_x_cond_winner <- (condorcet_winner_monadic A p x);
+    is_x_cond_winner \<leftarrow> (condorcet_winner_monadic A p x);
     RETURN (if (is_x_cond_winner) then 1 else 0)}"
 
 definition condorcet_ref :: "'a::{default, heap, hashable} Electoral_Module_Ref" where
   "condorcet_ref A pl  \<equiv> do {
-   scores <- (pre_compute_scores condorcet_score_ref A pl);
+   scores \<leftarrow> (pre_compute_scores condorcet_score_ref A pl);
    max_eliminator_ref scores A pl
 }"
 
@@ -35,11 +35,11 @@ lemma condorcet_score_ref_correct:
 
 lemma condorcet_ref_correct:          
   shows "(uncurry condorcet_ref, uncurry (RETURN oo condorcet)) \<in> 
-  ([\<lambda> (A, pl). finite_profile A
+  ([\<lambda> (A, pl). finite_profile A                         
             pl]\<^sub>f (\<langle>Id\<rangle>set_rel \<times>\<^sub>r profile_rel)
    \<rightarrow> \<langle>\<langle>Id\<rangle>set_rel \<times>\<^sub>r \<langle>Id\<rangle>set_rel \<times>\<^sub>r \<langle>Id\<rangle>set_rel\<rangle>nres_rel)"
-proof (unfold condorcet_ref_def comp_apply SPEC_eq_is_RETURN(2)[symmetric], 
-    intro frefI nres_relI, clarsimp simp add: set_rel_id prod_rel_id simp del : condorcet.simps,
+proof (unfold condorcet_ref_def, 
+    intro frefI nres_relI ,clarsimp simp del: max_eliminator.simps,
     rename_tac A pl pr)
   fix A :: "'a set"
   fix pl :: "'a Profile_List"
@@ -47,27 +47,10 @@ proof (unfold condorcet_ref_def comp_apply SPEC_eq_is_RETURN(2)[symmetric],
   assume prel: " (pl, pr) \<in> profile_rel"
   assume fina: "finite A"
   assume profp: "profile A pr"
-  from prel fina profp  have  precompcond: "pre_compute_scores condorcet_score_ref A pl
-  \<le> SPEC (\<lambda>map. map = pre_computed_map condorcet_score A pr)" using
-    condorcet_score_ref_correct compute_scores_correct
-    by metis
-  note maxelim = max_eliminator_ref_correct[where efn = condorcet_score and A = A and pl = pl
-      and pr = pr]
-  from fina prel this have mid: "(\<And>x. x = pre_computed_map condorcet_score A pr \<Longrightarrow>
-          max_eliminator_ref x A pl \<le> SPEC (\<lambda>x. x = max_eliminator condorcet_score A pr))"
-    by blast
-   have "pre_compute_scores condorcet_score_ref A pl \<bind> (\<lambda>scores. max_eliminator_ref scores A pl)
-       \<le> SPEC (\<lambda>x. x = condorcet A pr)"
-     unfolding condorcet.simps
-     apply refine_vcg
-     using precompcond  mid
-       SPEC_cons_rule[where m = "pre_compute_scores condorcet_score_ref A pl" and
-\<Psi> = "(\<lambda>scores. max_eliminator_ref scores A pl \<le> SPEC (\<lambda>x. x = max_eliminator condorcet_score A pr))"
-  and \<Phi> = "(\<lambda> map. map = (pre_computed_map condorcet_score A pr))"]
-     by blast 
-    thus " pre_compute_scores condorcet_score_ref A pl \<bind> (\<lambda>scores. max_eliminator_ref scores A pl)
-       \<le> RES {condorcet A pr}"
-    by (metis singleton_conv)
+  show " pre_compute_scores condorcet_score_ref A pl \<bind> (\<lambda>scores. max_eliminator_ref scores A pl)
+       \<le> RETURN (max_eliminator condorcet_score A pr)"
+     unfolding condorcet.simps RETURN_SPEC_conv
+     by (refine_vcg condorcet_score_ref_correct max_eliminator_ref_correct_default fina prel profp)
 qed
 
 sepref_definition condorcet_elim_sep is
@@ -76,19 +59,13 @@ sepref_definition condorcet_elim_sep is
    \<rightarrow>\<^sub>a (result_impl_assn nat_assn)"
   unfolding condorcet_ref_def  max_eliminator_ref_def condorcet_score_ref_def 
     less_eliminator_ref_def  elimination_module_ref_def[abs_def] eliminate_def[abs_def]
-    pre_compute_scores_def[abs_def] scoremax_def[abs_def] 
+    pre_compute_scores_def[abs_def] scoremax_def[abs_def] op_set_is_empty_def[symmetric]
   apply (rewrite in "FOREACH _ _ rewrite_HOLE" hm.fold_custom_empty)
   apply (rewrite in "FOREACH _ _ rewrite_HOLE" hs.fold_custom_empty)
   apply (rewrite in "FOREACH _ _ rewrite_HOLE" hs.fold_custom_empty)
-  apply (rewrite in "RETURN ({}, {}, rewrite_HOLE)" hs.fold_custom_empty) 
-  apply (rewrite in "RETURN ({}, rewrite_HOLE, _)" hs.fold_custom_empty) 
-  apply (rewrite in "RETURN ( rewrite_HOLE, _, _)" hs.fold_custom_empty) 
-  apply (rewrite in "_ \<bind> (\<lambda>(rej, def). if def = {} then RETURN (rewrite_HOLE, _, rej) 
-                                  else RETURN ({}, rej, def))" hs.fold_custom_empty)
-  apply (rewrite in "_ \<bind> (\<lambda>(rej, def). if def = {} then RETURN (_, rewrite_HOLE, rej) 
-                                  else RETURN ({}, rej, def))" hs.fold_custom_empty)
-  apply (rewrite in "_ \<bind> (\<lambda>(rej, def). if def = {} then RETURN (_, _, rej) 
-                                    else RETURN (rewrite_HOLE, rej, def))" hs.fold_custom_empty)
+  apply (rewrite in "RETURN (_, _, rewrite_HOLE)" hs.fold_custom_empty) 
+  apply (rewrite in "RETURN (_, rewrite_HOLE, _)" hs.fold_custom_empty) +
+  apply (rewrite in "RETURN ( rewrite_HOLE, _, _)" hs.fold_custom_empty)+ 
   apply sepref_dbg_keep
   done
 
